Fifo proven, start of Ltac rewrites.

Fifo/Proofs.v
@@ -6,364 +6,7 @@ Require Import StdLibKami.Fifo.Spec.
 Require Import Kami.GallinaModules.Relations.
 Require Import Kami.GallinaModules.AuxLemmas.
 Require Import Kami.GallinaModules.AuxTactics.
-
-Local Definition isEmpty_impl1 (varName : string) :=
-  (Read val : Bool <- varName; Ret (! Var type (SyntaxKind Bool) val))%kami_action.
-
-Local Definition isFull_impl1 (varName : string) :=
-  (Read val : Bool <- varName; Ret Var type (SyntaxKind Bool) val)%kami_action.
-
-Local Definition numFree_impl1 (varName : string) (size' : nat) :=
-  (Read val : Bool <- varName;
-   Ret (IF Var type (SyntaxKind Bool) val
-        then Const type (natToWord size' 0)
-        else Const type $ (1)%word))%kami_action.
-
-Local Definition first_impl1 (k : Kind) (bvarName dvarName : string)  :=
-(Read val : Bool <- bvarName;
- Read dat : k <- dvarName;
- Ret (STRUCT {"valid" ::= Var type (SyntaxKind Bool) val;
-              "data" ::= Var type (SyntaxKind k) dat}:
-      Expr type (SyntaxKind (Maybe k))))%kami_action.  
-
-Local Definition deq_impl1 (k : Kind) (bvarName dvarName : string) :=
-(Read val : Bool <- bvarName;
- Read dat : k <- dvarName;
- Write bvarName : Bool <- Const type false;
- Ret (STRUCT {"valid" ::= Var type (SyntaxKind Bool) val;
-              "data" ::= Var _ (SyntaxKind k) dat}:
-        Expr _ (SyntaxKind (Maybe k))))%kami_action.
-
-Local Definition enq_impl1 (k : Kind) (bvarName dvarName : string) (new : type k) :=
-  (Read val : Bool <- bvarName;
-   Read dat : k <- dvarName;
-   Write bvarName : Bool <- Const type true;
-   Write dvarName : k <-
-                    IF ! Var type (SyntaxKind Bool) val
-                    then Var _ (SyntaxKind k) new
-                    else Var _ _ dat;
-   Ret (! Var _ (SyntaxKind Bool) val))%kami_action.
-
-Local Definition flush_impl1 (varName : string) :=
-(Write varName : Bool <- Const type false; Retv)%kami_action.
-
-Local Lemma isEmpty1_Effectless varName val :
-  forall o reads upds calls retV,
-    NoDup (map fst o) ->
-    In (varName, existT _ (SyntaxKind Bool) val) o ->
-    SemAction o (isEmpty_impl1 varName) reads upds calls retV ->
-    upds = nil /\
-    calls = nil /\
-    retV = negb val.
-Proof.
-  unfold isEmpty_impl1; intros.
-  apply inversionSemAction in H1; dest; subst.
-  apply inversionSemAction in H2; dest; subst.
-  repeat split; auto.
-  enough ( x = val).
-  { subst; auto. }
-  specialize (NoDup_map_fst H H0 H1) as P; EqDep_subst; reflexivity.
-Qed.
-
-Local Lemma isEmpty1_Wb varName :
-  ActionWb [(varName, SyntaxKind Bool)] (isEmpty_impl1 varName).
-Proof.
-  unfold isEmpty_impl1.
-  repeat intro.
-  rewrite SubList_map_iff in H0; dest.
-  apply inversionSemAction in H1; dest; subst.
-  apply inversionSemAction in H3; dest; subst.
-  assert (SubList [(varName, existT (fullType type) (SyntaxKind Bool) x0)] o).
-  { repeat intro.
-    inv H3; [|inv H4]; assumption. }
-  specialize (SubList_chain H H0 H3) as P.
-  rewrite <- fst_getKindAttr in P.
-  setoid_rewrite H2 in P.
-  rewrite (P (eq_refl _)) in *.
-  split.
-  - exists [(varName, existT _ (SyntaxKind Bool) x0)]; repeat split; auto.
-    + apply SubList_refl.
-    + repeat econstructor.
-  - apply SubList_nil_l.
-Qed.
-
-Local Lemma isFull1_Effectless varName val :
-  forall o reads upds calls retV,
-    NoDup (map fst o) ->
-    In (varName, existT _ (SyntaxKind Bool) val) o ->
-    SemAction o (isFull_impl1 varName) reads upds calls retV ->
-    upds = nil /\
-    calls = nil /\
-    retV = val.
-Proof.
-  unfold isFull_impl1; intros.
-  apply inversionSemAction in H1; dest; subst.
-  apply inversionSemAction in H2; dest; subst.
-  repeat split; auto.
-  enough ( x = val).
-  { subst; auto. }
-  specialize (NoDup_map_fst H H0 H1) as P; EqDep_subst; reflexivity.
-Qed.
-
-Local Lemma isFull1_Wb varName :
-  ActionWb [(varName, SyntaxKind Bool)] (isFull_impl1 varName).
-Proof.
-  unfold isFull_impl1.
-  repeat intro.
-  rewrite SubList_map_iff in H0; dest.
-  apply inversionSemAction in H1; dest; subst.
-  apply inversionSemAction in H3; dest; subst.
-  assert (SubList [(varName, existT (fullType type) (SyntaxKind Bool) x0)] o).
-  { repeat intro.
-    inv H3; [|inv H4]; assumption. }
-  specialize (SubList_chain H H0 H3) as P.
-  rewrite <- fst_getKindAttr in P.
-  setoid_rewrite H2 in P.
-  rewrite (P (eq_refl _)) in *.
-  split.
-  - exists [(varName, existT _ (SyntaxKind Bool) x0)]; repeat split; auto.
-    + apply SubList_refl.
-    + repeat econstructor.
-  - apply SubList_nil_l.
-Qed.
-
-Local Lemma numFree1_Effectless varName size' val :
-  forall o reads upds calls retV,
-    NoDup (map fst o) ->
-    In (varName, existT _ (SyntaxKind Bool) val) o ->
-    SemAction o (numFree_impl1 varName size') reads upds calls retV ->
-    upds = nil /\
-    calls = nil /\
-    retV = (if val then (natToWord size' 0) else (natToWord size' 1)).
-Proof.
-  unfold numFree_impl1; intros.
-  apply inversionSemAction in H1; dest; subst.
-  apply inversionSemAction in H2; dest; subst.
-  repeat split; auto.
-  enough ( x = val).
-  { subst; auto. }
-  specialize (NoDup_map_fst H H0 H1) as P; EqDep_subst; reflexivity.
-Qed.
-
-Local Lemma numFree1_Wb varName size' :
-  ActionWb [(varName, SyntaxKind Bool)] (numFree_impl1 varName size').
-Proof.
-  unfold numFree_impl1.
-  repeat intro.
-  rewrite SubList_map_iff in H0; dest.
-  apply inversionSemAction in H1; dest; subst.
-  apply inversionSemAction in H3; dest; subst.
-  assert (SubList [(varName, existT (fullType type) (SyntaxKind Bool) x0)] o).
-  { repeat intro.
-    inv H3; [|inv H4]; assumption. }
-  specialize (SubList_chain H H0 H3) as P.
-  rewrite <- fst_getKindAttr in P.
-  setoid_rewrite H2 in P.
-  rewrite (P (eq_refl _)) in *.
-  split.
-  - exists [(varName, existT _ (SyntaxKind Bool) x0)]; repeat split; auto.
-    + apply SubList_refl.
-    + repeat econstructor.
-  - apply SubList_nil_l.
-Qed.
-
-Local Lemma first1_Effectless k bvarName dvarName bval dval:
-  forall o reads upds calls retV,
-    NoDup (map fst o) ->
-    In (bvarName, existT _ (SyntaxKind Bool) bval) o ->
-    In (dvarName, existT _ (SyntaxKind k) dval) o ->
-    SemAction o (first_impl1 k bvarName dvarName) reads upds calls retV ->
-    upds = nil /\
-    calls = nil /\
-    (retV F1 = bval) /\
-    (retV (FS F1) = dval).
-Proof.
-  unfold first_impl1; intros.
-  apply inversionSemAction in H2; dest; subst.
-  apply inversionSemAction in H3; dest; subst.
-  apply inversionSemAction in H4; dest; subst.
-  repeat split; auto.
-  - specialize (NoDup_map_fst H H0 H2) as P; EqDep_subst; reflexivity.
-  - specialize (NoDup_map_fst H H1 H3) as P; EqDep_subst; reflexivity.
-Qed.
-
-Local Lemma first1_Wb k bvarName dvarName :
-  ActionWb [(bvarName, SyntaxKind Bool); (dvarName, SyntaxKind k)]
-           (first_impl1 k bvarName dvarName).
-Proof.
-  unfold first_impl1.
-  repeat intro.
-  rewrite SubList_map_iff in H0; dest.
-  apply inversionSemAction in H1; dest; subst.
-  apply inversionSemAction in H3; dest; subst.
-  apply inversionSemAction in H4; dest; subst.
-  split; [|apply SubList_nil_l].
-  exists x.
-  assert (SubList [(bvarName, existT _ (SyntaxKind Bool) x0);
-                   (dvarName, existT _ (SyntaxKind k) x2)] o).
-  { repeat intro.
-    inv H4; [|inv H5; [|inv H4]]; assumption. }
-  specialize (SubList_chain H H0 H4) as P.
-  rewrite <- fst_getKindAttr in P.
-  setoid_rewrite H2 in P.
-  rewrite (P (eq_refl _)) in *.
-  repeat split; auto.
-  - apply SubList_refl.
-  - econstructor; eauto.
-    + left; reflexivity.
-    + econstructor; eauto.
-      * right; left; reflexivity.
-      * econstructor; eauto.
-Qed.
-
-Local Lemma deq1_Effectful k bvarName dvarName bval dval :
-  forall o reads upds calls retV,
-    NoDup (map fst o) ->
-    In (bvarName, existT _ (SyntaxKind Bool) bval) o ->
-    In (dvarName, existT _ (SyntaxKind k) dval) o ->
-    SemAction o (deq_impl1 k bvarName dvarName) reads upds calls retV ->
-    upds = [(bvarName, existT _ (SyntaxKind Bool) false)] /\
-    calls = nil /\
-    (retV F1 = bval) /\
-    (retV (FS F1) = dval).
-Proof.
-  unfold deq_impl1; intros.
-  apply inversionSemAction in H2; dest; subst.
-  apply inversionSemAction in H3; dest; subst.
-  apply inversionSemAction in H4; dest; subst.
-  apply inversionSemAction in H6; dest; subst.
-  repeat split; auto.
-  - specialize (NoDup_map_fst H H0 H2) as P; EqDep_subst; reflexivity.
-  - specialize (NoDup_map_fst H H1 H3) as P; EqDep_subst; reflexivity.
-Qed.
-
-Local Lemma deq1_Wb k bvarName dvarName :
-  ActionWb [(bvarName, SyntaxKind Bool); (dvarName, SyntaxKind k)]
-           (deq_impl1 k bvarName dvarName).
-Proof.
-  unfold deq_impl1.
-  repeat intro.
-  rewrite SubList_map_iff in H0; dest.
-  apply inversionSemAction in H1; dest; subst.
-  apply inversionSemAction in H3; dest; subst.
-  apply inversionSemAction in H4; dest; subst.
-  apply inversionSemAction in H6; dest; subst.
-  split.
-  - exists x.
-    assert (SubList [(bvarName, existT _ (SyntaxKind Bool) x0);
-                     (dvarName, existT _ (SyntaxKind k) x2)] o).
-    { repeat intro.
-      inv H6; [|inv H7; [|inv H6]]; assumption. }
-  specialize (SubList_chain H H0 H6) as P.
-  rewrite <- fst_getKindAttr in P.
-  setoid_rewrite H2 in P.
-  rewrite (P (eq_refl _)) in *.
-  repeat split; auto.
-    + apply SubList_refl.
-    + econstructor; eauto.
-      * left; reflexivity.
-      * econstructor; eauto.
-        -- right; left; reflexivity.
-        -- econstructor; eauto.
-           ++ left; auto.
-           ++ econstructor; eauto.
-  - repeat intro; inv H6;[|inv H7].
-    left; reflexivity.
-Qed.
-
-Local Lemma eqn1_Effectful k bvarName dvarName bval dval new:
-  forall o reads upds calls retV,
-    NoDup (map fst o) ->
-    In (bvarName, existT _ (SyntaxKind Bool) bval) o ->
-    In (dvarName, existT _ (SyntaxKind k) dval) o ->
-    SemAction o (enq_impl1 k bvarName dvarName new) reads upds calls retV ->
-    upds = [(bvarName, existT _ (SyntaxKind Bool) true);
-           (dvarName, existT _ (SyntaxKind k) 
-                             (if (negb bval)
-                             then new
-                             else dval))] /\
-    calls = nil /\
-    (retV = negb bval).
-Proof.
-  unfold enq_impl1; intros.
-  apply inversionSemAction in H2; dest; subst.
-  apply inversionSemAction in H3; dest; subst.
-  apply inversionSemAction in H4; dest; subst.
-  apply inversionSemAction in H6; dest; subst.
-  apply inversionSemAction in H8; dest; subst.
-  specialize (NoDup_map_fst H H0 H2) as P; EqDep_subst;
-    specialize (NoDup_map_fst H H1 H3) as P1; EqDep_subst.
-  repeat split; auto.
-Qed.
-
-Local Lemma eqn1_Wb k bvarName dvarName new:
-  ActionWb [(bvarName, SyntaxKind Bool); (dvarName, SyntaxKind k)]
-           (enq_impl1 k bvarName dvarName new).
-Proof.
-  unfold enq_impl1.
-  repeat intro.
-  rewrite SubList_map_iff in H0; dest.
-  apply inversionSemAction in H1; dest; subst.
-  apply inversionSemAction in H3; dest; subst.
-  apply inversionSemAction in H4; dest; subst.
-  apply inversionSemAction in H6; dest; subst.
-  apply inversionSemAction in H8; dest; subst.
-  split.
-  - exists x.
-    assert (SubList [(bvarName, existT _ (SyntaxKind Bool) x0);
-                     (dvarName, existT _ (SyntaxKind k) x2)] o).
-    { repeat intro.
-      inv H8; [|inv H9; [|inv H8]]; assumption. }
-  specialize (SubList_chain H H0 H8) as P.
-  rewrite <- fst_getKindAttr in P.
-  setoid_rewrite H2 in P.
-  rewrite (P (eq_refl _)) in *.
-  repeat split; auto.
-    + apply SubList_refl.
-    + econstructor; eauto.
-      * left; reflexivity.
-      * econstructor; eauto.
-        -- right; left; reflexivity.
-        -- econstructor; eauto.
-           ++ left; auto.
-           ++ econstructor; eauto.
-              ** right; left; reflexivity.
-              ** econstructor; reflexivity.
-  - repeat intro; inv H8;[|inv H9; [|inv H8]].
-    + left; reflexivity.
-    + right; left; reflexivity.
-Qed.
-
-Local Lemma flush1_Effectful varName :
-  forall o reads upds calls retV,
-    SemAction o (flush_impl1 varName) reads upds calls retV ->
-    upds = [(varName, existT _ (SyntaxKind Bool) false)] /\
-    calls = nil /\
-    (retV = WO).
-Proof.
-  unfold flush_impl1; intros.
-  apply inversionSemAction in H; dest; subst.
-  apply inversionSemAction in H1; dest; subst.
-  repeat split; auto.
-Qed.
-
-Local Lemma flush_Wb varName:
-  ActionWb [(varName, SyntaxKind Bool)]
-           (flush_impl1 varName).
-Proof.
-  unfold flush_impl1.
-  repeat intro.
-  rewrite SubList_map_iff in H0; dest.
-  apply inversionSemAction in H1; dest; subst.
-  apply inversionSemAction in H4; dest; subst.
-  split; [|apply SubList_refl].
-  exists x.
-  repeat split; auto.
-  - apply SubList_nil_l.
-  - repeat econstructor; eauto.
-    rewrite H2.
-    left; reflexivity.
-Qed.
+Require Import StdLibKami.RegArray.Proofs.
 
 Record FifoCorrect {FParams} (imp spec : @Fifo.Ifc.Ifc FParams) : Type :=
   {
@@ -384,41 +27,1135 @@ Record FifoCorrect {FParams} (imp spec : @Fifo.Ifc.Ifc FParams) : Type :=
     flushCorrect : EffectfulRelation fifoR (@flush _ imp type) (@flush _ spec type);
   }.
 
-Section Proofs.
+Section Proofs1.
   Context {ifcParams' : Fifo.Ifc.Params}.
-  Context `{implParams : @Impl.Params ifcParams'}.
-  Context `{specParams : @Spec.Params ifcParams'}.
-  Definition implFifo := @impl ifcParams' implParams.
-  Definition specFifo := @spec ifcParams'.
+  Variable Hsize1 : size = 1.
+  Variable impl1Params impl2Params : Impl.Params.
+  Local Definition fifoImpl1 := @Fifo.Impl.impl ifcParams' impl1Params.
+  Local Definition fifoImpl2 := @Fifo.Impl.impl ifcParams' impl2Params.
 
-  Variable implRegs : RegsT.
-  Variable deqVal enqVal : word (Fifo.Ifc.lgSize + 1).
-  Variable specRegs : RegT.
-  Variable listVal : list (type Fifo.Ifc.k).
-    
-  Record myFifoImplR (o_i o_s : RegsT) : Prop :=
+  Record myFifoImpl1R  (o_i o_s : RegsT) : Prop :=
     {
-      implRegVal : implRegs = [(Fifo.Impl.deqPtrName, existT _ (SyntaxKind (Bit (Fifo.Ifc.lgSize + 1))) deqVal);
-                              (Fifo.Impl.enqPtrName, existT _ (SyntaxKind (Bit (Fifo.Ifc.lgSize + 1))) enqVal)];
-      specRegVal : specRegs = (Fifo.Spec.listName, existT _ (Fifo.Spec.nlist type) listVal);
-      Ho_iCorrect : o_i = implRegs;
-      Ho_sCorrect : o_s = [specRegs];
-      Ho_iNoDup : NoDup (map fst o_i);
+      implRegs : RegsT;
+      fifo1_bval : bool;
+      fifo1_dval : type k;
+      implRegVal : implRegs = [(Fifo1.validRegName,
+                                existT _ (SyntaxKind Bool) fifo1_bval);
+                              (Fifo1.dataRegName,
+                               existT _ (SyntaxKind k) fifo1_dval)];
+      Ho_iCorrect1 : o_i = implRegs;
+      Ho_sCorrect1 : o_s = implRegs;
+      Ho_iNoDup1 : NoDup (map fst o_i);
+      Ho_sNoDup1 : NoDup (map fst o_s);
     }.
 
   Ltac Record_destruct :=
     match goal with
-    |[ H : myFifoImplR _ _ |- _] => destruct H
+    |[ H : myFifoImpl1R _ _ |- _] => destruct H
     end.
 
-  Goal FifoCorrect implFifo specFifo.
-    econstructor 1 with (fifoR := myFifoImplR) (fifoRegs := [(Fifo.Impl.deqPtrName, (SyntaxKind (Bit (Fifo.Ifc.lgSize + 1))));
-                                                             (Fifo.Impl.enqPtrName, (SyntaxKind (Bit (Fifo.Ifc.lgSize + 1))))]).
-    all : red; unfold implFifo, impl, specFifo, spec, regArray,
+  Goal FifoCorrect fifoImpl1 fifoImpl2.
+    rewrite <- Nat.eqb_eq in Hsize1.
+    all : econstructor 1 with (fifoR := myFifoImpl1R)
+                              (fifoRegs := [(Fifo1.validRegName,
+                                             SyntaxKind Bool);
+                                            (Fifo1.dataRegName,
+                                             SyntaxKind k)]).
+    all : red; unfold fifoImpl1, fifoImpl2, impl, spec, regArray,
                isEmpty, flush, enq, deq, numFree, isFull, first,
-               Impl.isEmpty, Impl.flush, Impl.enq, Impl.deq, Impl.numFree, Impl.isFull, Impl.first,
-               Spec.isEmpty, Spec.flush, Spec.enq, Spec.deq, Spec.numFree, Spec.isFull, Spec.first.
-    all : unfold Impl.isEmpty, Impl.fastModSize.
-    all : unfold Ifc.read; intros; try Record_destruct; hyp_consumer1.
+               Impl.isEmpty, Impl.flush, Impl.enq, Impl.deq, Impl.numFree,
+               Impl.isFull, Impl.first.
+    all : try rewrite Hsize1; unfold Fifo1.impl, Fifo1.isEmpty,
+                         Fifo1.isFull, Fifo1.flush, Fifo1.numFree, Fifo1.first,
+                         Fifo1.deq, Fifo1.enq; intros; try Record_destruct.
+    - hyp_consumer1; basic_goal_consumer.
+      inv H; [|inv H4; [|inv H]].
+      + apply inversionPair in H4; dest; EqDep_subst.
+        reflexivity.
+      + exfalso.
+        apply inversionPair in H; dest; rewrite H in *.
+        apply H0; reflexivity.
+    - hyp_consumer1.
+      rewrite in_map_iff in H1; dest.
+      apply inversionPair in H1; dest.
+      destruct x0, s0; simpl in *; subst.
+      goal_consumer2.
+      exact H3.
+    - hyp_consumer1.
+      basic_goal_consumer.
+      inv H; [|inv H4; [|inv H]].
+      + apply inversionPair in H4; dest; EqDep_subst.
+        reflexivity.
+      + exfalso.
+        apply inversionPair in H; dest; rewrite H in *.
+        apply H0; reflexivity.
+    - hyp_consumer1.
+      rewrite in_map_iff in H1; dest.
+      apply inversionPair in H1; dest.
+      destruct x0, s0; simpl in *; subst.
+      goal_consumer2.
+      exact H3.
+    - hyp_consumer1.
+      basic_goal_consumer.
+      inv H; [|inv H4; [|inv H]].
+      + apply inversionPair in H4; dest; EqDep_subst.
+        reflexivity.
+      + exfalso.
+        apply inversionPair in H; dest; rewrite H in *.
+        apply H0; reflexivity.
+    - hyp_consumer1.
+      rewrite in_map_iff in H0, H1; dest.
+      apply inversionPair in H1; dest.
+      destruct x0, s0; simpl in *; subst.
+      goal_consumer2.
+      exact H3.
+    - hyp_consumer1.
+      basic_goal_consumer.
+      inv H; [|inv H5; [|inv H]].
+      + inv H2; [|inv H; [|inv H2]].
+        * exfalso.
+          apply inversionPair in H; dest; rewrite H in *.
+          apply H0; reflexivity.
+        * apply inversionPair in H5; apply inversionPair in H2; dest; EqDep_subst.
+          reflexivity.
+      + exfalso.
+        apply inversionPair in H; dest; rewrite H in *.
+        apply H0; reflexivity.
+    - hyp_consumer1.
+      goal_consumer2.
+    - hyp_consumer1.
+      inv H; [|inv H6; [|inv H]].
+      + inv H2; [|inv H; [|inv H2]].
+        * exfalso.
+          apply inversionPair in H; dest; rewrite H in *.
+          apply H1; reflexivity.
+        * apply inversionPair in H6; dest.
+          apply inversionPair in H2; dest.
+          EqDep_subst.
+          basic_goal_consumer.
+          econstructor.
+          -- reflexivity.
+          -- destruct String.eqb eqn:G.
+             ++ exfalso.
+                rewrite String.eqb_eq in G.
+                rewrite G in *.
+                apply H1; reflexivity.
+             ++ reflexivity.
+          -- destruct String.eqb eqn:G.
+             ++ exfalso.
+                rewrite String.eqb_eq in G.
+                rewrite G in *.
+                apply H1; reflexivity.
+             ++ reflexivity.
+          -- destruct String.eqb eqn:G.
+             ++ exfalso.
+                rewrite String.eqb_eq in G.
+                rewrite G in *.
+                apply H1; reflexivity.
+             ++ basic_goal_consumer.
+          -- destruct String.eqb eqn:G.
+             ++ exfalso.
+                rewrite String.eqb_eq in G.
+                rewrite G in *.
+                apply H1; reflexivity.
+             ++ basic_goal_consumer.
+      + exfalso.
+          apply inversionPair in H; dest; rewrite H in *.
+          apply H1; reflexivity.
+    - hyp_consumer1.
+      goal_consumer2.
+    - hyp_consumer1.
+      inv H; [|inv H3; [|inv H]].
+      + inv H2; [|inv H; [|inv H2]].
+        * exfalso.
+          apply inversionPair in H; dest; rewrite H in *.
+          apply H1; reflexivity.
+        * apply inversionPair in H3; dest.
+          apply inversionPair in H2; dest.
+          EqDep_subst.
+          basic_goal_consumer.
+          econstructor.
+          -- reflexivity.
+          -- destruct String.eqb eqn:G.
+             ++ simpl in G.
+                rewrite String.eqb_eq in G.
+                destruct String.eqb eqn:G0 in G; simpl in G.
+                ** exfalso.
+                   rewrite G in *.
+                   apply H1; reflexivity.
+                ** simpl.
+                   rewrite eqb_sym in G0.
+                   rewrite G0.
+                   reflexivity.
+             ++ simpl in *.
+                rewrite String.eqb_neq in G.
+                rewrite eqb_sym at 1.
+                rewrite eqb_sym in G.
+                destruct String.eqb eqn: G0; auto.
+                ** exfalso.
+                   rewrite String.eqb_eq in G0.
+                   rewrite G0 in *.
+                   apply H1; reflexivity.
+                ** exfalso.
+                   apply G; reflexivity.
+          -- destruct String.eqb eqn:G.
+             ++ simpl in G.
+                rewrite String.eqb_eq in G.
+                destruct String.eqb eqn:G0 in G; simpl in G.
+                ** exfalso.
+                   rewrite G in *.
+                   apply H1; reflexivity.
+                ** simpl.
+                   rewrite eqb_sym in G0.
+                   rewrite G0.
+                   reflexivity.
+             ++ simpl in *.
+                rewrite String.eqb_neq in G.
+                destruct String.eqb eqn:G0 in G; simpl in G.
+                ** exfalso.
+                   rewrite String.eqb_eq in G0.
+                   apply G; rewrite G0; reflexivity.
+                ** exfalso.
+                   apply G; reflexivity.
+          -- destruct String.eqb eqn:G.
+             ++ rewrite String.eqb_eq in G.
+                destruct String.eqb eqn:G0; simpl in *.
+                ** exfalso.
+                   rewrite G in *; apply H1; reflexivity.
+                ** rewrite eqb_sym in G0.
+                   rewrite G0; simpl.
+                   repeat econstructor; intro P; inv P; [|inv H3].
+                   apply H1; rewrite H3; reflexivity.
+             ++ rewrite String.eqb_neq in G.
+                destruct String.eqb eqn:G0; simpl in *.
+                ** exfalso.
+                   rewrite String.eqb_eq in G0.
+                   rewrite G0 in *; apply H1; reflexivity.
+                ** rewrite eqb_sym in G0.
+                   rewrite G0; simpl.
+                   repeat econstructor; intro P; inv P; [|inv H3].
+                   apply H1; rewrite H3; reflexivity.
+          --  destruct String.eqb eqn:G.
+             ++ rewrite String.eqb_eq in G.
+                destruct String.eqb eqn:G0; simpl in *.
+                ** exfalso.
+                   rewrite G in *; apply H1; reflexivity.
+                ** rewrite eqb_sym in G0.
+                   rewrite G0; simpl.
+                   repeat econstructor; intro P; inv P; [|inv H3].
+                   apply H1; rewrite H3; reflexivity.
+             ++ rewrite String.eqb_neq in G.
+                destruct String.eqb eqn:G0; simpl in *.
+                ** exfalso.
+                   rewrite String.eqb_eq in G0.
+                   rewrite G0 in *; apply H1; reflexivity.
+                ** rewrite eqb_sym in G0.
+                   rewrite G0; simpl.
+                   repeat econstructor; intro P; inv P; [|inv H3].
+                   apply H1; rewrite H3; reflexivity.
+      + exfalso.
+        apply inversionPair in H; dest; rewrite H in *.
+        apply H1; reflexivity.
+    - hyp_consumer1.
+      goal_consumer2.
+    - hyp_consumer1.
+      basic_goal_consumer.
+      destruct String.eqb eqn:G.
+      + exfalso.
+        rewrite String.eqb_eq in G.
+        apply H0; rewrite G; reflexivity.
+      + rewrite String.eqb_neq in G.
+        econstructor; simpl; eauto; repeat normalize_key_concl; auto.
+  Qed.
+End Proofs1.
+
+(* Section Proofs2. *)
+(*   Context {ifcParams' : Fifo.Ifc.Params}. *)
+(*   Variable Hsize1 : size <> 1. *)
+(*   Variable impl1Params impl2Params : Impl.Params. *)
+(*   Local Definition regArray1 := @regArray ifcParams' impl1Params. *)
+(*   Local Definition regArray2 := @regArray ifcParams' impl2Params. *)
+(*   Local Definition fifoImpl1' := @Fifo.Impl.impl ifcParams' impl1Params. *)
+(*   Local Definition fifoImpl2' := @Fifo.Impl.impl ifcParams' impl2Params. *)
+  
+(*   Variable HRegArrayCorrect : RegArrayCorrect regArray1 regArray2. *)
+
+(*   Record myFifoImplR (regArrayR : RegsT -> RegsT -> Prop) regArrayRegs *)
+(*          (o_i o_s : RegsT) : Prop := *)
+(*     {    *)
+(*       implRegs : RegsT; *)
+(*       enqVal : word (Fifo.Ifc.lgSize + 1); *)
+(*       deqVal : word (Fifo.Ifc.lgSize + 1); *)
+(*       regArray1Regs : RegsT; *)
+(*       regArray2Regs : RegsT; *)
+(*       implRegVal : implRegs = [(Fifo.Impl.deqPtrName, *)
+(*                                 existT _ (SyntaxKind (Bit (Fifo.Ifc.lgSize + 1))) deqVal); *)
+(*                               (Fifo.Impl.enqPtrName, *)
+(*                                existT _ (SyntaxKind (Bit (Fifo.Ifc.lgSize + 1))) enqVal)]; *)
+(*       Ho_iCorrect : o_i = implRegs ++ regArray1Regs; *)
+(*       Ho_sCorrect : o_s = implRegs ++ regArray2Regs; *)
+(*       Ho_iNoDup : NoDup (map fst o_i); *)
+(*       Ho_sNoDup : NoDup (map fst o_s); *)
+(*       HRegArrayRegs : getKindAttr regArray1Regs = regArrayRegs; *)
+(*       HRegArray : regArrayR regArray1Regs regArray2Regs; *)
+(*     }. *)
+
+(*   Ltac Record_destruct := *)
+(*     match goal with *)
+(*     |[ H : myFifoImplR _ _ _ _ |- _] => destruct H *)
+(*     end. *)
+  
+(*   Goal FifoCorrect fifoImpl1' fifoImpl2'. *)
+(*     destruct HRegArrayCorrect. *)
+(*     rewrite <- Nat.eqb_neq in Hsize1. *)
+(*     all : econstructor 1 with (fifoR := myFifoImplR regArrayR regArrayRegs) *)
+(*                         (fifoRegs := [(Fifo.Impl.deqPtrName, *)
+(*                                        (SyntaxKind (Bit (Fifo.Ifc.lgSize + 1)))); *)
+(*                                       (Fifo.Impl.enqPtrName, *)
+(*                                        (SyntaxKind (Bit (Fifo.Ifc.lgSize + 1))))] *)
+(*                                        ++ regArrayRegs). *)
+(*     all : red; unfold fifoImpl1', fifoImpl2', impl, spec, regArray, *)
+(*                isEmpty, flush, enq, deq, numFree, isFull, first, *)
+(*                Impl.isEmpty, Impl.flush, Impl.enq, Impl.deq, Impl.numFree, *)
+(*                Impl.isFull, Impl.first. *)
+(*     all : try rewrite Hsize1; unfold Fifo1.impl, Fifo1.isEmpty, *)
+(*                          Fifo1.isFull, Fifo1.flush, Fifo1.numFree, Fifo1.first, *)
+(*                          Fifo1.deq, Fifo1.enq; intros; try Record_destruct. *)
+(*     all : unfold regArray1, Impl.isEmpty in *. *)
+(*     - hyp_consumer1. *)
+(*       repeat normalize_key_hyps. *)
+(*       repeat clean_useless_hyp. *)
+(*       basic_goal_consumer. *)
+(*       rewrite in_app_iff in H2, H. *)
+(*       specialize (H8 Impl.deqPtrName) as P. *)
+(*       specialize (H8 Impl.enqPtrName) as P0. *)
+(*       destruct H, H2. *)
+(*       + inv H; [| inv H4; [exfalso; apply H0; *)
+(*                            apply inversionPair in H; *)
+(*                            dest; rewrite H; reflexivity| inv H]]. *)
+(*         inv H2; [exfalso; apply H0; *)
+(*                  apply inversionPair in H; *)
+(*                  dest; rewrite H; reflexivity| inv H;[| inv H2]]. *)
+(*         apply inversionPair in H4; apply inversionPair in H2; dest; EqDep_subst. *)
+(*         reflexivity. *)
+(*       + apply (in_map fst) in H2. *)
+(*         destruct P0; try tauto. *)
+(*         exfalso; apply H4. *)
+(*         right; left; reflexivity. *)
+(*       + apply (in_map fst) in H. *)
+(*         destruct P; try tauto. *)
+(*         exfalso; apply H4. *)
+(*         left; reflexivity. *)
+(*       + apply (in_map fst) in H. *)
+(*         destruct P; try tauto. *)
+(*         exfalso; apply H4. *)
+(*         left; reflexivity. *)
+(*     - hyp_consumer1. *)
+(*       rewrite SubList_map_iff in H1; dest. *)
+(*       repeat goal_consumer. *)
+(*       + instantiate (1 := [(Impl.deqPtrName, existT _ (SyntaxKind (Bit (lgSize + 1))) x); *)
+(*                            (Impl.enqPtrName, existT _ (SyntaxKind (Bit (lgSize + 1))) x1)] *)
+(*                             ++ x0). *)
+(*         goal_consumer2. *)
+(*       + goal_consumer2. *)
+(*       + goal_consumer2. *)
+(*       + goal_consumer2. *)
+(*       + goal_consumer2. *)
+(*       + goal_consumer2. *)
+(*       + goal_consumer2. *)
+(*       + goal_consumer2. *)
+(*       + goal_consumer2. *)
+(*       + goal_consumer2. *)
+(*       + goal_consumer2. *)
+(*       + goal_consumer2. *)
+(*       + goal_consumer2. *)
+(*     - hyp_consumer1. *)
+(*       repeat clean_useless_hyp. *)
+(*       basic_goal_consumer. *)
+(*       rewrite in_app_iff in H2, H. *)
+(*       specialize (H8 Impl.deqPtrName) as P. *)
+(*       specialize (H8 Impl.enqPtrName) as P0. *)
+(*       destruct H, H2. *)
+(*       + inv H; [| inv H4; [exfalso; apply H0; *)
+(*                            apply inversionPair in H; *)
+(*                            dest; rewrite H; reflexivity| inv H]]. *)
+(*         inv H2; [exfalso; apply H0; *)
+(*                  apply inversionPair in H; *)
+(*                  dest; rewrite H; reflexivity| inv H;[| inv H2]]. *)
+(*         apply inversionPair in H4; apply inversionPair in H2; dest; EqDep_subst. *)
+(*         reflexivity. *)
+(*       + apply (in_map fst) in H2. *)
+(*         destruct P0; try tauto. *)
+(*         exfalso; apply H4. *)
+(*         right; left; reflexivity. *)
+(*       + apply (in_map fst) in H. *)
+(*         destruct P; try tauto. *)
+(*         exfalso; apply H4. *)
+(*         left; reflexivity. *)
+(*       + apply (in_map fst) in H. *)
+(*         destruct P; try tauto. *)
+(*         exfalso; apply H4. *)
+(*         left; reflexivity. *)
+(*     - hyp_consumer1. *)
+(*       rewrite SubList_map_iff in H1; dest. *)
+(*       repeat goal_consumer. *)
+(*       + instantiate (1 := [(Impl.deqPtrName, existT _ (SyntaxKind (Bit (lgSize + 1))) x); *)
+(*                            (Impl.enqPtrName, existT _ (SyntaxKind (Bit (lgSize + 1))) x1)] *)
+(*                             ++ x0). *)
+(*         goal_consumer2. *)
+(*       + goal_consumer2. *)
+(*       + goal_consumer2. *)
+(*       + goal_consumer2. *)
+(*       + goal_consumer2. *)
+(*       + goal_consumer2. *)
+(*       + goal_consumer2. *)
+(*       + goal_consumer2. *)
+(*       + goal_consumer2. *)
+(*       + goal_consumer2. *)
+(*       + goal_consumer2. *)
+(*       + goal_consumer2. *)
+(*       + goal_consumer2. *)
+(*     - hyp_consumer1. *)
+(*       repeat clean_useless_hyp. *)
+(*       basic_goal_consumer. *)
+(*       rewrite in_app_iff in H2, H. *)
+(*       specialize (H8 Impl.deqPtrName) as P. *)
+(*       specialize (H8 Impl.enqPtrName) as P0. *)
+(*       destruct H, H2. *)
+(*       + inv H; [| inv H4; [exfalso; apply H0; *)
+(*                            apply inversionPair in H; *)
+(*                            dest; rewrite H; reflexivity| inv H]]. *)
+(*         inv H2; [exfalso; apply H0; *)
+(*                  apply inversionPair in H; *)
+(*                  dest; rewrite H; reflexivity| inv H;[| inv H2]]. *)
+(*         apply inversionPair in H4; apply inversionPair in H2; dest; EqDep_subst. *)
+(*         reflexivity. *)
+(*       + apply (in_map fst) in H2. *)
+(*         destruct P0; try tauto. *)
+(*         exfalso; apply H4. *)
+(*         right; left; reflexivity. *)
+(*       + apply (in_map fst) in H. *)
+(*         destruct P; try tauto. *)
+(*         exfalso; apply H4. *)
+(*         left; reflexivity. *)
+(*       + apply (in_map fst) in H. *)
+(*         destruct P; try tauto. *)
+(*         exfalso; apply H4. *)
+(*         left; reflexivity. *)
+(*     - hyp_consumer1. *)
+(*       rewrite SubList_map_iff in H1; dest. *)
+(*       repeat goal_consumer. *)
+(*       + instantiate (1 := [(Impl.deqPtrName, existT _ (SyntaxKind (Bit (lgSize + 1))) x); *)
+(*                            (Impl.enqPtrName, existT _ (SyntaxKind (Bit (lgSize + 1))) x1)] *)
+(*                             ++ x0). *)
+(*         goal_consumer2. *)
+(*       + goal_consumer2. *)
+(*       + goal_consumer2. *)
+(*       + goal_consumer2. *)
+(*       + goal_consumer2. *)
+(*       + goal_consumer2. *)
+(*       + goal_consumer2. *)
+(*       + goal_consumer2. *)
+(*       + goal_consumer2. *)
+(*       + goal_consumer2. *)
+(*       + goal_consumer2. *)
+(*       + goal_consumer2. *)
+(*       + goal_consumer2. *)
+(*     - unfold regArray1, Impl.isEmpty in *. *)
+(*       hyp_consumer1. *)
+(*       rewrite in_app_iff in H7, H9, H5. *)
+(*       specialize (H8 Impl.deqPtrName) as P. *)
+(*       specialize (H8 Impl.enqPtrName) as P0. *)
+      
+(*       destruct H7; [|exfalso; apply (in_map fst) in H2; simpl in *; tauto]. *)
+(*       destruct H9; [|exfalso; apply (in_map fst) in H3; simpl in *; tauto]. *)
+(*       destruct H5; [|exfalso; apply (in_map fst) in H4; simpl in *; tauto]. *)
+(*       inv H2; [|inv H5; [exfalso; apply H; *)
+(*                          apply inversionPair in H2; *)
+(*                          dest; rewrite H2; reflexivity| inv H2]]. *)
+(*       inv H3; [exfalso; apply H; *)
+(*                apply inversionPair in H2; *)
+(*                dest; rewrite H2; reflexivity|inv H2; [|inv H3]]. *)
+(*       inv H4; [|inv H2; [exfalso; apply H; *)
+(*                          apply inversionPair in H4; *)
+(*                          dest; rewrite H2; reflexivity| inv H4]]. *)
+(*       apply inversionPair in H5; dest. *)
+(*       apply inversionPair in H3; dest. *)
+(*       apply inversionPair in H2; dest. *)
+(*       destruct P, P0; simpl in H10, H11; try tauto. *)
+(*       EqDep_subst. *)
+(*       repeat clean_useless_hyp. *)
+(*       basic_goal_consumer; auto. *)
+(*       + eapply SemActionExpand; [|apply HSemAction_s]. *)
+(*         rewrite Permutation.Permutation_app_comm. *)
+(*         apply SubList_app_r, SubList_refl. *)
+(*       + reflexivity. *)
+(*       + reflexivity. *)
+(*     - unfold regArray1, Impl.isEmpty in *. *)
+(*       hyp_consumer1. *)
+(*       specialize (NoDup_map_fst H H9 H7) as TMP; EqDep_subst. *)
+(*       goal_consumer2. *)
+(*       eapply SemActionExpand;[|apply H10]. *)
+(*       rewrite Permutation.Permutation_app_comm. *)
+(*       apply SubList_app_r, SubList_refl. *)
+(*     - unfold regArray1, Impl.isEmpty in *. *)
+(*       hyp_consumer1. *)
+(*       specialize (H9 Impl.deqPtrName) as P; simpl in P. *)
+(*       rewrite in_app_iff in H14. *)
+(*       destruct H14; [|apply (in_map fst) in H; simpl in H; try tauto]. *)
+(*       inv H;[|inv H0; [exfalso; apply inversionPair in H; dest; *)
+(*                        apply H2; rewrite H; reflexivity|inv H]]. *)
+(*       apply inversionPair in H0; dest; EqDep_subst. *)
+(*       destruct H10;[|apply (in_map fst) in H0; destruct H0; try tauto;  *)
+(*                      simpl in H0, H2; symmetry in H0; tauto]. *)
+(*       apply inversionPair in H0; dest; EqDep_subst. *)
+(*       rewrite in_app_iff in H12. *)
+(*       destruct H12 as [S|S]; [|apply (in_map fst) in S; simpl in S; try tauto]. *)
+(*       inversion_clear S as [S0|S0];[|inversion_clear S0 as [S1|S1]; *)
+(*                                      [exfalso; apply inversionPair in S1; dest; apply H2; *)
+(*                                       rewrite H5; reflexivity *)
+(*                                      |inv S1]]. *)
+(*       apply inversionPair in S0; dest; EqDep_subst. *)
+(*       specialize (H9 Impl.enqPtrName) as P0; simpl in P0. *)
+(*       rewrite in_app_iff in H16. *)
+(*       destruct H16 as [S|S]; [|apply (in_map fst) in S; simpl in S; try tauto]. *)
+(*       inversion_clear S as [S0|S0]; *)
+(*         [exfalso; apply inversionPair in S0; dest; *)
+(*          apply H2; rewrite H6; reflexivity| inversion_clear S0 as [S1|S1];[|inv S1]]. *)
+(*       apply inversionPair in S1; dest; EqDep_subst. *)
+(*       repeat clean_useless_hyp. *)
+(*       clear P P0. *)
+(*       goal_consumer2. *)
+(*       + instantiate (1 := nil). *)
+(*         repeat intro. *)
+(*         inv H. *)
+(*       + basic_goal_consumer. *)
+(*       + econstructor. *)
+(*         * reflexivity. *)
+(*         * basic_goal_consumer. *)
+(*           destruct String.eqb eqn:G. *)
+(*           -- exfalso. *)
+(*              rewrite String.eqb_eq in G; simpl in G. *)
+(*              apply H2. *)
+(*              rewrite G; reflexivity. *)
+(*           -- reflexivity. *)
+(*         * basic_goal_consumer. *)
+(*           destruct String.eqb eqn:G. *)
+(*           -- exfalso. *)
+(*              rewrite String.eqb_eq in G; simpl in G. *)
+(*              apply H2. *)
+(*              rewrite G; reflexivity. *)
+(*           -- reflexivity. *)
+(*         * basic_goal_consumer. *)
+(*         * basic_goal_consumer. *)
+(*         * rewrite oneUpdRegs_notIn; auto. *)
+(*           repeat intro; simpl in H. *)
+(*           specialize (H9 Impl.deqPtrName); destruct H9; try tauto. *)
+(*           apply H0; left; reflexivity. *)
+(*         * repeat rewrite oneUpdRegs_notIn; auto. *)
+(*           -- intro; simpl in H. *)
+(*              specialize (H4 Impl.deqPtrName); destruct H4; try tauto. *)
+(*              apply H0; left; reflexivity. *)
+(*           -- intro; simpl in H. *)
+(*              specialize (H9 Impl.deqPtrName); destruct H9; try tauto. *)
+(*              apply H0; left; reflexivity. *)
+(*     - unfold regArray1, Impl.isEmpty in *. *)
+(*       hyp_consumer1. *)
+(*       specialize (NoDup_map_fst H H14 H16) as TMP; EqDep_subst. *)
+(*       specialize (NoDup_map_fst H H14 H12) as TMP; EqDep_subst. *)
+(*       repeat clean_useless_hyp. *)
+(*       simpl in H1. *)
+(*       goal_consumer2. *)
+(*       basic_goal_consumer. *)
+(*     - hyp_consumer1. *)
+(*       + rewrite in_app_iff in H, H7, H9. *)
+(*         specialize (H11 Impl.enqPtrName) as P. *)
+(*         specialize (H11 Impl.deqPtrName) as P0. *)
+(*         simpl in P, P0. *)
+(*         destruct H as [S|S];[|apply (in_map fst) in S; simpl in S; tauto]. *)
+(*         inversion_clear S as [S0|S0]; [exfalso; apply inversionPair in S0; dest; *)
+(*                                        apply H2; rewrite H; reflexivity| *)
+(*                                       inversion_clear S0 as [S|S]; [|inv S]]. *)
+(*         apply inversionPair in S; dest; EqDep_subst. *)
+(*         destruct H7 as [S|S];[|apply (in_map fst) in S; simpl in S; tauto]. *)
+(*         inversion_clear S as [S0|S0]; [|inversion_clear S0 as [S|S]; *)
+(*                                         [exfalso; apply inversionPair in S as [G ?]; dest; *)
+(*                                          apply H2; rewrite G; reflexivity|inv S]]. *)
+(*         apply inversionPair in S0; dest; EqDep_subst. *)
+(*         destruct H9 as [S|S];[|apply (in_map fst) in S; simpl in S; tauto]. *)
+(*         inversion_clear S as [S0|S0]; [exfalso; apply inversionPair in S0 as [G ?]; dest; *)
+(*                                        apply H2; rewrite G; reflexivity| *)
+(*                                        inversion_clear S0 as [S|S]; [|inv S]]. *)
+(*         apply inversionPair in S; dest; EqDep_subst. *)
+(*         repeat clean_useless_hyp. *)
+(*         clear P P0. *)
+(*         goal_consumer2. *)
+(*         * instantiate (1 := upds_s). *)
+(*           repeat intro. *)
+(*           simpl in H. *)
+(*           specialize (SemActionUpdSub HSemAction_s) as P. *)
+(*           apply (in_map fst) in H. *)
+(*           apply  (SubList_map fst) in P. *)
+(*           repeat rewrite fst_getKindAttr in P. *)
+(*           specialize (P _ H). *)
+(*           specialize (H4 Impl.enqPtrName) as P0; simpl in P0; tauto. *)
+(*         * goal_consumer2. *)
+(*         * econstructor. *)
+(*           -- reflexivity. *)
+(*           -- basic_goal_consumer. *)
+(*              destruct String.eqb eqn:G. *)
+(*              ++ exfalso. *)
+(*                 rewrite String.eqb_eq in G. *)
+(*                 apply H2; rewrite G; reflexivity. *)
+(*              ++ rewrite doUpdReg_notIn; eauto. *)
+(*                 apply (SubList_map fst) in H23. *)
+(*                 repeat rewrite fst_getKindAttr in H23. *)
+(*                 intro. *)
+(*                 specialize (H23 _ H). *)
+(*                 specialize (H11 Impl.deqPtrName) as P; simpl in P, H23; tauto. *)
+(*           -- basic_goal_consumer. *)
+(*              ++ destruct String.eqb eqn:G. *)
+(*                 ** exfalso. *)
+(*                    rewrite String.eqb_eq in G; simpl in G. *)
+(*                    apply H2; rewrite G; reflexivity. *)
+(*                 ** apply SemActionUpdSub in HSemAction_s. *)
+(*                    rewrite doUpdReg_notIn; auto. *)
+(*                    repeat intro. *)
+(*                    apply (SubList_map fst) in HSemAction_s. *)
+(*                    repeat rewrite fst_getKindAttr in HSemAction_s. *)
+(*                    specialize (HSemAction_s _ H); simpl in HSemAction_s. *)
+(*                    specialize (H4 Impl.deqPtrName) as P; simpl in P; tauto. *)
+(*              ++ rewrite doUpdReg_notIn; auto. *)
+(*                 intro. *)
+(*                 apply SemActionUpdSub in HSemAction_s. *)
+(*                 apply (SubList_map fst) in HSemAction_s. *)
+(*                 repeat rewrite fst_getKindAttr in HSemAction_s. *)
+(*                 specialize (HSemAction_s _ H); simpl in HSemAction_s. *)
+(*                 specialize (H4 Impl.enqPtrName) as P; simpl in P; tauto. *)
+(*           -- basic_goal_consumer. *)
+(*           -- basic_goal_consumer. *)
+(*           -- rewrite oneUpdRegs_notIn. *)
+(*              ++ apply doUpdReg_preserves_getKindAttr; auto. *)
+(*              ++ intro G; simpl in G. *)
+(*                 specialize (H11 Impl.enqPtrName) as P; simpl in P; tauto. *)
+(*           -- repeat rewrite oneUpdRegs_notIn; auto. *)
+(*              ++ intro G; simpl in G. *)
+(*                 specialize (H4 Impl.enqPtrName) as P; simpl in P; tauto. *)
+(*              ++ intro G; simpl in G. *)
+(*                 specialize (H11 Impl.enqPtrName) as P; simpl in P; tauto. *)
+(*       + rewrite in_app_iff in H, H7, H9. *)
+(*         specialize (H8 Impl.enqPtrName) as P. *)
+(*         specialize (H8 Impl.deqPtrName) as P0. *)
+(*         simpl in P, P0. *)
+(*         destruct H as [S|S];[|apply (in_map fst) in S; simpl in S; tauto]. *)
+(*         inversion_clear S as [S0|S0]; [exfalso; apply inversionPair in S0; dest; *)
+(*                                        apply H0; rewrite H; reflexivity| *)
+(*                                       inversion_clear S0 as [S|S]; [|inv S]]. *)
+(*         apply inversionPair in S; dest; EqDep_subst. *)
+(*         destruct H7 as [S|S];[|apply (in_map fst) in S; simpl in S; tauto]. *)
+(*         inversion_clear S as [S0|S0]; [|inversion_clear S0 as [S|S]; *)
+(*                                         [exfalso; apply inversionPair in S as [G ?]; dest; *)
+(*                                          apply H0; rewrite G; reflexivity|inv S]]. *)
+(*         apply inversionPair in S0; dest; EqDep_subst. *)
+(*         destruct H9 as [S|S];[|apply (in_map fst) in S; simpl in S; tauto]. *)
+(*         inversion_clear S as [S0|S0]; [exfalso; apply inversionPair in S0 as [G ?]; dest; *)
+(*                                        apply H0; rewrite G; reflexivity| *)
+(*                                        inversion_clear S0 as [S|S]; [|inv S]]. *)
+(*         apply inversionPair in S; dest; EqDep_subst. *)
+(*         repeat clean_useless_hyp. *)
+(*         clear P P0. *)
+(*         goal_consumer2. *)
+(*         * econstructor. *)
+(*           -- reflexivity. *)
+(*           -- basic_goal_consumer. *)
+(*           -- basic_goal_consumer. *)
+(*           -- basic_goal_consumer. *)
+(*           -- basic_goal_consumer. *)
+(*           -- basic_goal_consumer. *)
+(*           -- basic_goal_consumer. *)
+(*     - hyp_consumer1; specialize (NoDup_map_fst H H2 H11) as TMP; EqDep_subst *)
+(*       ; repeat clean_useless_hyp. *)
+(*       + goal_consumer2. *)
+(*         eapply (SemActionExpand); [|apply H12]. *)
+(*         basic_goal_consumer. *)
+(*       + rewrite SubList_map_iff in H1; dest. *)
+(*         split; [|goal_consumer2]. *)
+(*         exists ([(Impl.deqPtrName, existT _ (SyntaxKind (Bit (lgSize + 1))) x8); *)
+(*                        (Impl.enqPtrName, existT _ (SyntaxKind (Bit (lgSize + 1))) x10)] *)
+(*                   ++ x). *)
+(*         goal_consumer2. *)
+(*     - hyp_consumer1. *)
+(*       basic_goal_consumer. *)
+(*       econstructor. *)
+(*       + reflexivity. *)
+(*       + destruct String.eqb eqn:G. *)
+(*         * simpl in G; rewrite String.eqb_eq in G. *)
+(*           destruct String.eqb eqn:G0. *)
+(*           -- exfalso. *)
+(*              apply H0; simpl in G; simpl. *)
+(*              rewrite G; reflexivity. *)
+(*           -- simpl. *)
+(*              rewrite eqb_sym in G0. *)
+(*              rewrite G0. *)
+(*              repeat rewrite oneUpdRegs_notIn. *)
+(*              ++ reflexivity. *)
+(*              ++ intro. *)
+(*                 specialize (H10 Impl.enqPtrName) as P. *)
+(*                 simpl in P, H2; tauto. *)
+(*              ++ intro. *)
+(*                 specialize (H10 Impl.deqPtrName) as P. *)
+(*                 simpl in P, H2; tauto. *)
+(*              ++ intro. *)
+(*                 specialize (H10 Impl.enqPtrName) as P. *)
+(*                 simpl in P, H2; tauto. *)
+(*         * rewrite String.eqb_neq in G; simpl in G. *)
+(*           destruct String.eqb eqn:G0. *)
+(*           -- exfalso. *)
+(*              rewrite String.eqb_eq in G0; simpl in G0. *)
+(*              apply H0; simpl; rewrite G0; reflexivity. *)
+(*           -- exfalso; apply G; reflexivity. *)
+(*       + simpl. *)
+(*         destruct String.eqb eqn:G. *)
+(*         * rewrite String.eqb_eq in G. *)
+(*           destruct String.eqb eqn:G0. *)
+(*           -- exfalso. *)
+(*              simpl in G. *)
+(*              apply H0; rewrite G; reflexivity. *)
+(*           -- rewrite eqb_sym in G0. *)
+(*              rewrite G0. *)
+(*              repeat rewrite oneUpdRegs_notIn. *)
+(*              ++ reflexivity. *)
+(*              ++ simpl; intro. *)
+(*                 specialize (H5 Impl.enqPtrName) as P. *)
+(*                 simpl in P. *)
+(*                 tauto. *)
+(*              ++ simpl; intro. *)
+(*                 specialize (H5 Impl.deqPtrName) as P. *)
+(*                 simpl in P. *)
+(*                 tauto. *)
+(*              ++ simpl; intro. *)
+(*                 specialize (H5 Impl.enqPtrName) as P. *)
+(*                 simpl in P. *)
+(*                 tauto. *)
+(*         * rewrite String.eqb_neq in G. *)
+(*           destruct String.eqb eqn:G0. *)
+(*           -- exfalso. *)
+(*              rewrite String.eqb_eq in G0. *)
+(*              apply G; rewrite G0; reflexivity. *)
+(*           -- exfalso; apply G; reflexivity. *)
+(*       + simpl. *)
+(*         destruct String.eqb eqn:G. *)
+(*         * rewrite String.eqb_eq in G. *)
+(*           destruct String.eqb eqn:G0. *)
+(*           -- exfalso. *)
+(*              apply H0; simpl in G; rewrite G; reflexivity. *)
+(*           -- rewrite eqb_sym in G0. *)
+(*              rewrite G0. *)
+(*              repeat rewrite oneUpdRegs_notIn. *)
+(*              ++ basic_goal_consumer. *)
+(*                 ** intro. *)
+(*                    specialize (H10 Impl.deqPtrName) as P. *)
+(*                    simpl in P; tauto. *)
+(*                 ** intro. *)
+(*                    specialize (H10 Impl.enqPtrName) as P. *)
+(*                    simpl in P; tauto. *)
+(*              ++ intro. *)
+(*                 specialize (H10 Impl.enqPtrName) as P. *)
+(*                 simpl in P; tauto. *)
+(*              ++ intro. *)
+(*                 specialize (H10 Impl.deqPtrName) as P. *)
+(*                 simpl in P; tauto. *)
+(*              ++ intro. *)
+(*                 specialize (H10 Impl.enqPtrName) as P. *)
+(*                 simpl in P; tauto. *)
+(*         * rewrite String.eqb_neq in G. *)
+(*           destruct String.eqb eqn:G0. *)
+(*           -- exfalso. *)
+(*              rewrite String.eqb_eq in G0. *)
+(*              apply G; rewrite G0; reflexivity. *)
+(*           -- exfalso. *)
+(*              apply G; reflexivity. *)
+(*       + simpl. *)
+(*         destruct String.eqb eqn:G. *)
+(*         * rewrite String.eqb_eq in G. *)
+(*           destruct String.eqb eqn:G0. *)
+(*           -- exfalso. *)
+(*              apply H0; simpl in G; rewrite G; reflexivity. *)
+(*           -- rewrite eqb_sym in G0. *)
+(*              rewrite G0. *)
+(*              repeat rewrite oneUpdRegs_notIn. *)
+(*              ++ basic_goal_consumer. *)
+(*                 ** intro. *)
+(*                    specialize (H5 Impl.deqPtrName) as P. *)
+(*                    simpl in P; tauto. *)
+(*                 ** intro. *)
+(*                    specialize (H5 Impl.enqPtrName) as P. *)
+(*                    simpl in P; tauto. *)
+(*              ++ intro. *)
+(*                 specialize (H5 Impl.enqPtrName) as P. *)
+(*                 simpl in P; tauto. *)
+(*              ++ intro. *)
+(*                 specialize (H5 Impl.deqPtrName) as P. *)
+(*                 simpl in P; tauto. *)
+(*              ++ intro. *)
+(*                 specialize (H5 Impl.enqPtrName) as P. *)
+(*                 simpl in P; tauto. *)
+(*         * rewrite String.eqb_neq in G. *)
+(*           destruct String.eqb eqn:G0. *)
+(*           -- exfalso. *)
+(*              rewrite String.eqb_eq in G0. *)
+(*              apply G; rewrite G0; reflexivity. *)
+(*           -- exfalso. *)
+(*              apply G; reflexivity. *)
+(*       + reflexivity. *)
+(*       + assumption. *)
+(*         Unshelve. *)
+(*         all: eauto. *)
+(*         exact nil. *)
+(*         exact WO. *)
+(*         exact nil. *)
+(*         exact WO. *)
+(*   Qed. *)
+
+(* End Proofs2. *)
+
+
+Section Proofs2'.
+  Context {ifcParams' : Fifo.Ifc.Params}.
+  Variable Hsize1 : size <> 1.
+  Variable impl1Params impl2Params : Impl.Params.
+  Local Definition regArray1 := @regArray ifcParams' impl1Params.
+  Local Definition regArray2 := @regArray ifcParams' impl2Params.
+  Local Definition fifoImpl1' := @Fifo.Impl.impl ifcParams' impl1Params.
+  Local Definition fifoImpl2' := @Fifo.Impl.impl ifcParams' impl2Params.
+  
+  Variable HRegArrayCorrect : RegArrayCorrect regArray1 regArray2.
+
+  Record myFifoImplR (regArrayR : RegsT -> RegsT -> Prop) regArrayRegs
+         (o_i o_s : RegsT) : Prop :=
+    {   
+      implRegs : RegsT;
+      enqVal : word (Fifo.Ifc.lgSize + 1);
+      deqVal : word (Fifo.Ifc.lgSize + 1);
+      regArray1Regs : RegsT;
+      regArray2Regs : RegsT;
+      implRegVal : implRegs = [(Fifo.Impl.deqPtrName,
+                                existT _ (SyntaxKind (Bit (Fifo.Ifc.lgSize + 1))) deqVal);
+                              (Fifo.Impl.enqPtrName,
+                               existT _ (SyntaxKind (Bit (Fifo.Ifc.lgSize + 1))) enqVal)];
+      Ho_iCorrect : o_i = implRegs ++ regArray1Regs;
+      Ho_sCorrect : o_s = implRegs ++ regArray2Regs;
+      Ho_iNoDup : NoDup (map fst o_i);
+      Ho_sNoDup : NoDup (map fst o_s);
+      HRegArrayRegs : getKindAttr regArray1Regs = regArrayRegs;
+      HRegArray : regArrayR regArray1Regs regArray2Regs;
+    }.
+
+  Ltac Record_destruct :=
+    match goal with
+    |[ H : myFifoImplR _ _ _ _ |- _] => destruct H
+    end.
+
+
+  Ltac normalize_key_hyps1 :=
+    match goal with
+    | [ H : context [map fst (_ ++ _)] |- _] => rewrite map_app in H
+    | [ H : forall _, (~In _ (map fst ?l1)) \/ (~In _ (map fst ?l2)) |- _]
+      => fold (DisjKey l1 l2) in H
+    | [ H : NoDup (_ ++ _) |- _]
+      => rewrite (NoDup_app_Disj_iff string_dec) in H; destruct H as [? [? ?]]
+    | [ H : DisjKey (_ ++ _) _ |- _] => rewrite DisjKey_app_split_l in H; destruct H as [? ?]
+    | [ H : DisjKey _ (_ ++ _) |- _] => rewrite DisjKey_app_split_r in H; destruct H as [? ?]
+    | [ H : ~In _ (_ ++ _) |- _] => rewrite (nIn_app_iff string_dec) in H; destruct H as [? ?]
+    | [ H : DisjKey (_ :: _) _ |- _] => rewrite DisjKey_cons_l_str in H; destruct H as [? ?]
+    | [ H : DisjKey _ (_ :: _) |- _] => rewrite DisjKey_cons_r_str in H; destruct H as [? ?]
+    end.
+
+  Ltac normalize_key_hyps2 :=
+    match goal with
+    | [ H : context [map fst (_ :: _)] |- _] => rewrite map_cons in H
+    | [ H : context [map fst nil] |- _] => rewrite map_nil in H
+    | [ H : NoDup (_ :: _) |- _] => rewrite NoDup_cons_iff in H; destruct H as [? ?]
+    | [ H : key_not_In _ (_ :: _) |- _] => rewrite key_not_In_cons in H; destruct H as [? ?]
+    | [ H : ~In _ (_ :: _) |- _] => rewrite not_in_cons in H; destruct H as [? ?]
+    end.
+
+  Ltac normalize_key_hyps' :=
+    repeat normalize_key_hyps1;
+    repeat normalize_key_hyps2;
+    cbn [fst] in *;
+    repeat clean_useless_hyp.
+  
+  Ltac my_simpl_solver' :=
+    match goal with
+    | [ H : ?P |- ?P] => apply H
+    | [ |- DisjKey nil _] => apply DisjKey_nil_l
+    | [ |- DisjKey _ nil] => apply DisjKey_nil_r
+    | [ |- ?a = ?a] => reflexivity
+    | [ |- True] => apply I
+    | [ |- NoDup nil] => constructor
+    | [ |- ~In _ nil] => intro; my_simpl_solver
+    | [ H : False |- _] => exfalso; apply H
+    | [ H : ?a <> ?a |- _] => exfalso; apply H; reflexivity
+    | [ H : In _ nil |- _] => inversion H
+    | [ |- SubList nil _ ] => apply SubList_nil_l
+    | [ |- SubList ?a ?a] => apply SubList_refl
+    | [ |- ?a = ?b] => is_evar a; reflexivity
+    | [ |- ?a = ?b] => is_evar b; reflexivity
+    | [ H: ?a = ?b |- _] => discriminate
+    | [H1 : ?a = ?b,
+            H2 : ?a <> ?b |- _] => exfalso; apply H2; rewrite H1; reflexivity
+    | [H1 : ?a = ?b,
+            H2 : ?b <> ?a |- _] => exfalso; apply H2; rewrite H1; reflexivity
+    | [|- nil = ?l1 ++ ?l2] => symmetry; apply (app_eq_nil l1 l2); split
+    | [|- ?l1 ++ ?l2 = nil] => apply (app_eq_nil l1 l2); split
+    end.
+  
+  Ltac goal_consumer2' :=
+    repeat goal_split
+    ; repeat goal_body
+    ; repeat normal_solver2
+    ; repeat my_risky_solver
+    ; repeat normal_solver2.
+
+  Ltac normalize_key_concl1 :=
+    match goal with
+    | [|- context [map fst (_ ++ _)]] => rewrite map_app               
+    | [|- forall _, (~In _ (map fst ?l1)) \/ (~In _ (map fst ?l2))]
+      => fold (DisjKey l1 l2)
+    | [ |- NoDup (_ ++ _)] => rewrite (NoDup_app_Disj_iff string_dec); repeat split
+    | [ |- DisjKey (_ ++ _) _] => rewrite DisjKey_app_split_l; split
+    | [ |- DisjKey _ (_ ++ _)] => rewrite DisjKey_app_split_r; split
+    | [ |- ~In _ (_ ++ _)] => rewrite (nIn_app_iff string_dec); split
+    | [ |- DisjKey (_ :: _) _] => rewrite DisjKey_cons_l_str; split
+    | [ |- DisjKey _ (_ :: _)] => rewrite DisjKey_cons_r_str; split
+    end.
+
+  Ltac normalize_key_concl2 :=
+    match goal with
+    | [ |- context [map fst (_ :: _)]] => rewrite map_cons
+    | [ |- context [map fst nil]] => rewrite map_nil
+    | [ |- NoDup (_ :: _)] => rewrite NoDup_cons_iff; split
+    | [ |- key_not_In _ (_ :: _)] => rewrite key_not_In_cons; split
+    | [ |- ~In _ (_ :: _)] => rewrite not_in_cons; split
+    | [ |- key_not_In _ ?l] =>
+      match l with
+      | _ => has_evar l; idtac
+      | _ => rewrite key_not_In_fst
+      end
+    | [ |- ~In _ (_ :: _)] => rewrite not_in_cons; split
+    | [ |- ~In _ (_ ++ _)] => rewrite (nIn_app_iff string_dec); split
+    end.
+
+  Ltac normalize_key_concl' :=
+    repeat normalize_key_concl1;
+    repeat normalize_key_concl2;
+    cbn [fst];
+    repeat (solve_keys || my_simpl_solver).
+  
+  Ltac resolve_wb'' :=
+    let HNoDup := fresh "H" in
+    let HSubList := fresh "H" in
+    match goal with
+    | [HSemAction1 :SemAction ?o1 ?a_i _ _ _ _,
+                    HActionWb : ActionWb ?myR ?a_i |- _] =>
+      assert (NoDup (map fst o1)) as HNoDup
+      ;[repeat normalize_key_concl'
+       | assert (SubList myR (getKindAttr o1)) as HSubList
+         ;[clear HNoDup HSemAction1
+           ; repeat normalize_sublist_l
+           ; sublist_sol
+          | specialize (HActionWb _ _ _ _ _ HNoDup HSubList HSemAction1)
+            as [[? [? [? [? ?]]]] ?]
+            ; try resolve_sublist2
+            ; clear HSemAction1 HNoDup HSubList]]
+    | [HSemAction1 : SemAction ?o1 (?a_i _) _ _ _ _,
+                     HActionWb : forall _, ActionWb ?myR (?a_i _) |- _] =>
+      assert (NoDup (map fst o1)) as HNoDup
+      ;[repeat normalize_key_concl'
+       | assert (SubList myR (getKindAttr o1)) as HSubList
+         ;[clear HNoDup HSemAction1
+           ; repeat normalize_sublist_l
+           ; sublist_sol
+          | specialize (HActionWb _ _ _ _ _ _ HNoDup HSubList HSemAction1)
+            as [[? [? [? [? ?]]]] ?]
+            ; try resolve_sublist2
+            ; clear HSemAction1 HNoDup HSubList]]
+    | [HSemAction1 : SemAction ?o1 (?a_i _ _ _ _ _) _ _ _ _,
+                     HActionWb :  forall _ _ _ _, ActionWb ?myR (?a_i _ _ _ _ _)|- _] =>
+      assert (NoDup (map fst o1)) as HNoDup
+      ;[repeat normalize_key_concl'
+       | assert (SubList myR (getKindAttr o1)) as HSubList
+         ;[clear HNoDup HSemAction1
+          | specialize (HActionWb _ _ _ _ _ _ _ _ _ HNoDup HSubList HSemAction1)
+            as [[? [? [? [? ?]]]] ?]
+            ; try resolve_sublist2
+            ; clear HSemAction1 HNoDup HSubList]]
+    end.
+  
+  Ltac resolve_wb_testing :=
+    let HNoDup := fresh "H" in
+    let HSubList := fresh "H" in
+    match goal with
+    | [HSemAction1 :SemAction ?o1 ?a_i _ _ _ _,
+                    HActionWb : ActionWb ?myR ?a_i |- _] =>
+      idtac "found 1 :" HSemAction1 HActionWb
+    | [HSemAction1 : SemAction ?o1 (?a_i _) _ _ _ _,
+                     HActionWb : forall _, ActionWb ?myR (?a_i _) |- _] =>
+      idtac "found 2 :" HSemAction1 HActionWb;
+      assert (NoDup (map fst o1)) as HNoDup
+      ;[|]
+    | [HSemAction1 : SemAction ?o1 (?a_i _ _ _ _ _) _ _ _ _,
+                     HActionWb :  forall _ _ _ _, ActionWb ?myR (?a_i _ _ _ _ _)|- _] =>
+      idtac "found 3 :" HSemAction1 HActionWb
+    end.
+  
+  Ltac hyp_consumer1' :=
+    repeat mySubst;
+    normalize_key_hyps';
+    repeat (repeat main_body
+            ; repeat mySubst
+            ; repeat (my_simplifier; repeat clean_useless_hyp)
+            ; repeat mySubst
+            ; repeat normalize_key_hyps
+            ; repeat (my_simplifier; repeat clean_useless_hyp)
+            ; repeat (resolve_wb''; repeat clean_useless_hyp)
+            ; repeat resolve_rel'
+            ; repeat mySubst
+            ; repeat (my_simplifier ; repeat clean_useless_hyp))
+    ; repeat my_simpl_solver'.
+
+  Ltac goal_body' :=
+    match goal with
+    | [ |- SemAction _ (Return _) _ _ _ _ ] => econstructor 10
+    | [ |- SemAction _ (MCall _ _ _ _) _ _ _ _] => econstructor 1
+    | [ |- SemAction _ (LetAction _ _) _ _ _ _] => econstructor 3
+    | [ |- SemAction _ (ReadReg _ _ _) _ _ _ _] => econstructor 5
+    | [ |- SemAction _ (WriteReg _ _ _) _ _ _ _] => econstructor 6
+    | [ |- SemAction _ (IfElse _ _ _ _) _ _ _ _]
+      => eapply SemAction_if_split
+         ;[ find_if_inside| | | | ]
+    | [ |- SemAction _ (LetExpr _ _) _ _ _ _] => econstructor 2
+    | [ |- SemAction _ (ReadNondet _ _) _ _ _ _] => econstructor 4
+    | [ |- SemAction _ (Sys _ _) _ _ _ _] => econstructor 9
+    | [ H : SemAction ?o ?a _ _ _ _ |- SemAction ?o ?a _ _ _ _]
+      => apply H
+    | [ H : SemAction ?o1 ?a _ _ _ _ |- SemAction ?o2 ?a _ _ _ _]
+      => eapply SemActionExpand;[| apply H; sublist_sol]
+    end.
+
+  Ltac doUpdRegs_red' :=  
+    repeat 
+      (match goal with
+       | [ |- context [ doUpdRegs nil _]] => rewrite doUpdRegs_nil
+       | [ |- context [ doUpdReg nil _]] => rewrite doUpdReg_nil
+       | |- context [ oneUpdRegs ?r ?o ] =>
+         let TMP := fresh "H" in
+         assert (TMP : ~ In (fst r) (map fst o));
+         [ repeat
+             match goal with
+             | |- context [ map fst (doUpdRegs _ _) ] => rewrite doUpdRegs_preserves_keys
+             end; solve_keys
+         | rewrite (oneUpdRegs_notIn _ _ TMP); clear TMP ]
+       | |- context [ doUpdReg ?u ?r ] =>
+         let TMP := fresh "H" in
+         assert (TMP : ~ In (fst r) (map fst u));
+         [ repeat
+             match goal with
+             | |- context [ map fst (doUpdRegs _ _) ] => rewrite doUpdRegs_preserves_keys
+             end; solve_keys
+         | rewrite (doUpdReg_notIn _ _ TMP); clear TMP ]; cbn[fst]
+       end);
+    repeat
+      match goal with
+      | |- context [oneUpdReg _ _ ] => cbv [oneUpdReg fst]
+      | [|- context [?a =? ?a]] => rewrite eqb_refl 
+      | H : fst ?r1 = fst ?r2
+        |- context [fst ?r1 =? fst ?r2] =>
+        rewrite (proj2 (String.eqb_eq (fst r1) (fst r2)) H)
+      | H : fst ?r2 = fst ?r1
+        |- context [fst ?r1 =? fst ?r2] =>
+        rewrite eqb_sym, (proj2 (String.eqb_eq (fst r2) (fst r1)) H)
+      | H : fst ?r1 <> fst ?r2
+        |- context [fst ?r1 =? fst ?r2] =>
+        rewrite (proj2 (String.eqb_neq (fst r1) (fst r2)) H)
+      | H : fst ?r2 <> fst ?r1
+        |- context [fst ?r1 =? fst ?r2] =>
+        rewrite eqb_sym, (proj2 (String.eqb_neq (fst r2) (fst r1)) H) 
+      | H : ?a = ?b
+        |- context [?a =? ?b] =>
+        rewrite (proj2 (String.eqb_eq a b) H)
+      | H : ?b = ?a
+        |- context [?a =? ?b] =>
+        rewrite eqb_sym, (proj2 (String.eqb_eq b a) H)
+      | H : ?a <> ?b
+        |- context [?a =? ?b] =>
+        rewrite (proj2 (String.eqb_neq a b) H)
+      | H : ?b <> ?a
+        |- context [?a =? ?b] =>
+        rewrite eqb_sym, (proj2 (String.eqb_neq b a) H)
+      end.
+
+  Ltac basic_goal_consumer' :=
+    repeat (repeat goal_split
+            ; repeat goal_body'
+            ; repeat normal_solver)
+    ; repeat (repeat doUpdRegs_simpl
+              ; doUpdRegs_red'
+              ; repeat normal_solver).
+  (*
+            ; repeat normal_solver
+            ; repeat my_risky_solver
+            ; repeat gka_doUpdReg_red
+            ; repeat normal_solver)*)
+  Goal FifoCorrect fifoImpl1' fifoImpl2'.
+    destruct HRegArrayCorrect.
+    rewrite <- Nat.eqb_neq in Hsize1.
+    all : econstructor 1 with (fifoR := myFifoImplR regArrayR regArrayRegs)
+                        (fifoRegs := [(Fifo.Impl.deqPtrName,
+                                       (SyntaxKind (Bit (Fifo.Ifc.lgSize + 1))));
+                                      (Fifo.Impl.enqPtrName,
+                                       (SyntaxKind (Bit (Fifo.Ifc.lgSize + 1))))]
+                                       ++ regArrayRegs).
+    all : red; unfold fifoImpl1', fifoImpl2', impl, spec, regArray,
+               isEmpty, flush, enq, deq, numFree, isFull, first,
+               Impl.isEmpty, Impl.flush, Impl.enq, Impl.deq, Impl.numFree,
+               Impl.isFull, Impl.first.
+    all : try rewrite Hsize1; unfold Fifo1.impl, Fifo1.isEmpty,
+                         Fifo1.isFull, Fifo1.flush, Fifo1.numFree, Fifo1.first,
+                         Fifo1.deq, Fifo1.enq; intros; try Record_destruct.
+    all : unfold regArray1, Impl.isEmpty in *.
+    - hyp_consumer1'.
+      basic_goal_consumer.
+    - admit.
+    - hyp_consumer1'.
+      basic_goal_consumer.
+    - admit.
+    - hyp_consumer1'.
+      basic_goal_consumer.
+    - admit.
+    - hyp_consumer1'.
+      basic_goal_consumer'; repeat my_simpl_solver'.
+    - admit.
+    - hyp_consumer1'.
+      basic_goal_consumer'.
+      econstructor; eauto; normalize_key_concl'.
+    - admit.
+    - hyp_consumer1'.
+      + basic_goal_consumer'.
+        econstructor; eauto; normalize_key_concl'; repeat rewrite doUpdRegs_preserves_keys;
+          normalize_key_concl'.
+        gka_doUpdReg_red; normal_solver; auto.
+      + basic_goal_consumer'.
+        econstructor; eauto; normalize_key_concl'.
+    - admit.
+    - hyp_consumer1'.
+      cbn [fst] in *.
+      basic_goal_consumer'.
+      econstructor; eauto; normalize_key_concl'.
+      Unshelve.
+      all : eauto.
+      exact nil.
+      exact WO.
   Admitted.
-End Proofs.
+End Proofs2'.
